cleanup

dimsum/iris/sim.v
@@ -2,28 +2,33 @@ From iris.bi Require Import fixpoint.
 From iris.proofmode Require Export proofmode.
 From iris.base_logic.lib Require Export fancy_updates.
 From iris.base_logic.lib Require Export ghost_var.
+From dimsum.core Require Import axioms.
 From dimsum.core Require Export module trefines.
 From dimsum.core.iris Require Export ord_later.
 Set Default Proof Using "Type".
 
 (** * mstate_var *)
-Class mstateG (Σ : gFunctors) (S : Type) := MStateGS {
-  mstate_ghost_varG :: ghost_varG Σ S;
+Record mstate_var_type : TypeOrdinal := MstateVar {
+  mstate_var_ty : TypeState;
+  mstate_val_val : mstate_var_ty;
 }.
-Global Hint Mode mstateG - ! : typeclass_instances.
+Class mstateG (Σ : gFunctors) := MStateGS {
+  mstate_ghost_varG :: ghost_varG Σ mstate_var_type;
+}.
+Global Hint Mode mstateG - : typeclass_instances.
 
-Definition mstateΣ S : gFunctors :=
-  #[ ghost_varΣ S ].
+Definition mstateΣ : gFunctors :=
+  #[ ghost_varΣ mstate_var_type ].
 
-Global Instance subG_mstateΣ Σ S :
-  subG (mstateΣ S) Σ → mstateG Σ S.
+Global Instance subG_mstateΣ Σ :
+  subG mstateΣ Σ → mstateG Σ.
 Proof. solve_inG. Qed.
 
-Definition mstate_var {Σ S} `{!mstateG Σ S} (γ : gname) (s : S) :=
-  ghost_var γ (1/2) s.
+Definition mstate_var {Σ} {S : TypeState} `{!mstateG Σ} (γ : gname) (s : S) :=
+  ghost_var γ (1/2) (MstateVar _ s).
 
-Definition mstate_var_full {Σ S} `{!mstateG Σ S} (γ : gname) :=
-  (∃ s : S, ghost_var γ 1 s)%I.
+Definition mstate_var_full {Σ} {S : TypeState} `{!mstateG Σ} (γ : gname) :=
+  (∃ s : S, ghost_var γ 1 (MstateVar _ s))%I.
 
 Notation "γ '⤳' σ " := (mstate_var γ σ)
    (at level 20, format "γ  '⤳'  σ") : bi_scope.
@@ -33,7 +38,7 @@ Notation "γ '⤳@{' S '}' '-' " := (mstate_var_full (S:=S) γ)
    (at level 20, only parsing) : bi_scope.
 
 Section mstate_var.
-  Context {Σ S} `{!mstateG Σ S}.
+  Context {Σ} {S : TypeState} `{!mstateG Σ}.
   Implicit Types (σ : S).
 
   Lemma mstate_var_alloc `{!Inhabited S}:
@@ -43,8 +48,8 @@ Section mstate_var.
   Lemma mstate_var_merge γ σ1 σ2 :
     γ ⤳ σ1 -∗ γ ⤳ σ2 -∗ ⌜σ1 = σ2⌝ ∗ γ ⤳@{S} -.
   Proof.
-    iIntros "H1 H2". iDestruct (ghost_var_agree with "[$] [$]") as %->. iSplit; [done|].
-    iExists _. iFrame.
+    iIntros "H1 H2". iDestruct (ghost_var_agree with "[$] [$]") as %[=].
+    simplify_K. iSplit; [done|]. iExists _. iFrame.
   Qed.
 
   Lemma mstate_var_split γ σ :
@@ -60,16 +65,18 @@ Global Typeclasses Opaque mstate_var mstate_var_full.
 Class dimsumPreG (Σ : gFunctors) := DimsumPreG {
   dimsum_pre_invG :: invGpreS Σ;
   dimsum_pre_ord_laterG :: ord_laterPreG Σ;
+  dimsum_pre_mstateG :: mstateG Σ;
 }.
 
 Class dimsumGS (Σ : gFunctors) := DimsumGS {
   dimsum_invGS :: invGS_gen HasNoLc Σ;
   dimsum_ord_laterGS :: ord_laterGS Σ;
+  dimsum_mstateG :: mstateG Σ;
 }.
 Global Opaque dimsum_invGS.
 
 Definition dimsumΣ : gFunctors :=
-  #[ ord_laterΣ; invΣ ].
+  #[ ord_laterΣ; invΣ; mstateΣ ].
 
 Global Instance subG_dimsumΣ Σ :
   subG (dimsumΣ) Σ → dimsumPreG Σ.
@@ -557,18 +564,15 @@ Section sim.
     σ_t ≈{m_t}≈>ₜ sim_tgtP σ_s -∗ σ_t ⪯{m_t, m_s} σ_s.
   Proof. iIntros "?". by rewrite sim_unfold. Qed.
 
-  Definition sim_src_constP `{!mstateG Σ (m_state m_t)} `{!mstateG Σ (option EV)}
-    (γσ_t γκ : gname) :
+  Definition sim_src_constP (γσ_t γκ : gname) :
     option EV → m_state m_s → iProp Σ :=
     λ κ' σ_s', (∀ κ σ_t', γκ ⤳ κ -∗ γσ_t ⤳ σ_t' -∗ ⌜κ = κ'⌝ ∗ σ_t' ⪯{m_t, m_s} σ_s')%I.
 
-  Definition sim_tgt_constP
-    `{!mstateG Σ (m_state m_s)} `{!mstateG Σ (m_state m_t)} `{!mstateG Σ (option EV)}
-    (γσ_t γσ_s γκ : gname) :
+  Definition sim_tgt_constP (γσ_t γσ_s γκ : gname) :
     option EV → m_state m_t → iProp Σ :=
     λ κ σ_t', (∀ σ_s, γσ_s ⤳ σ_s -∗ γκ ⤳ κ -∗ γσ_t ⤳ σ_t' -∗ σ_s ≈{m_s}≈>ₛ sim_src_constP γσ_t γκ)%I.
 
-  Lemma sim_tgt_constP_intro_weak γσ_t γσ_s γκ σ_t σ_s `{!mstateG Σ (m_state m_s)} `{!mstateG Σ (m_state m_t)} `{!mstateG Σ (option EV)} :
+  Lemma sim_tgt_constP_intro_weak γσ_t γσ_s γκ σ_t σ_s :
     γσ_t ⤳@{m_state m_t} - -∗
     γσ_s ⤳ σ_s -∗
     γκ ⤳@{option EV} - -∗
@@ -586,7 +590,7 @@ Section sim.
     iApply ("Ht" with "[$] [$]").
   Qed.
 
-  Lemma sim_tgt_constP_intro γσ_t γσ_s γκ σ_t σ_s `{!mstateG Σ (m_state m_s)} `{!mstateG Σ (m_state m_t)} `{!mstateG Σ (option EV)} :
+  Lemma sim_tgt_constP_intro γσ_t γσ_s γκ σ_t σ_s :
     γσ_t ⤳@{m_state m_t} - -∗
     γσ_s ⤳@{m_state m_s} - -∗
     γκ ⤳@{option EV} - -∗
@@ -599,8 +603,7 @@ Section sim.
     by iApply (sim_tgt_constP_intro_weak with "[$] [$] [$]").
   Qed.
 
-  Lemma sim_tgt_constP_elim γσ_t γσ_s γκ σ_t σ_s κ
-    `{!mstateG Σ (m_state m_s)} `{!mstateG Σ (m_state m_t)} `{!mstateG Σ (option EV)} :
+  Lemma sim_tgt_constP_elim γσ_t γσ_s γκ σ_t σ_s κ :
     γσ_s ⤳ σ_s -∗
     (γσ_s ⤳@{m_state m_s} - -∗ γσ_t ⤳ σ_t -∗ γκ ⤳ κ -∗ σ_s ≈{m_s}≈>ₛ sim_src_constP γσ_t γκ) -∗
     sim_tgt_constP γσ_t γσ_s γκ κ σ_t.
@@ -610,8 +613,7 @@ Section sim.
     iApply ("HC" with "[$] [$] [$]").
   Qed.
 
-  Lemma sim_src_constP_elim γσ_t γκ σ_t σ_s κ κ'
-    `{!mstateG Σ (m_state m_s)} `{!mstateG Σ (m_state m_t)} `{!mstateG Σ (option EV)} :
+  Lemma sim_src_constP_elim γσ_t γκ σ_t σ_s κ κ' :
     γσ_t ⤳ σ_t -∗
     γκ ⤳ κ -∗
     (γσ_t ⤳@{m_state m_t} - -∗ γκ ⤳@{option EV} - -∗ ⌜κ = κ'⌝ ∗ σ_t ⪯{m_t, m_s} σ_s) -∗
@@ -623,12 +625,24 @@ Section sim.
     iApply ("HC" with "[$] [$]").
   Qed.
 
+  Lemma sim_src_constP_next γσ_t γσ_s γκ σ_t σ_s κ κ' :
+    γσ_t ⤳ σ_t -∗
+    γκ ⤳ κ -∗
+    γσ_s ⤳@{m_state m_s} - -∗
+    ⌜κ = κ'⌝ -∗
+    (γσ_s ⤳ σ_s -∗ σ_t ≈{m_t}≈>ₜ sim_tgt_constP γσ_t γσ_s γκ) -∗
+    sim_src_constP γσ_t γκ κ' σ_s.
+  Proof.
+    iIntros "?? Hσ_s -> HC". iApply (sim_src_constP_elim with "[$] [$]"). iIntros "Hσ_t Hκ".
+    iSplit; [done|]. iApply (sim_tgt_constP_intro with "Hσ_t Hσ_s Hκ HC").
+  Qed.
+
 End sim.
 
 Theorem sim_adequacy Σ EV (m_t m_s : module EV) `{!dimsumPreG Σ} `{!VisNoAng (m_trans m_s)} :
   (∀ `{Hinv : !invGS_gen HasNoLc Σ} `{Hord : !ord_laterGS Σ},
     ⊢ |={⊤}=>
-       let _ : dimsumGS Σ := DimsumGS _ _ _
+       let _ : dimsumGS Σ := DimsumGS _ _ _ _
        in
        m_init m_t ⪯{m_trans m_t, m_trans m_s} m_init m_s ) →
   trefines m_t m_s.
@@ -637,7 +651,7 @@ Proof.
   eapply uPred.pure_soundness. apply (step_fupdN_soundness_no_lc _ 0 0) => ? /=. simpl in *. iIntros "_".
   iMod (ord_later_alloc n) as (?) "Ha". iDestruct (ord_later_ctx_alloc with "Ha") as "#?".
   iMod Hsim as "Hsim".
-  clear Hsim. set (X := DimsumGS _ _ _ : dimsumGS Σ).
+  clear Hsim. set (X := DimsumGS _ _ _ _ : dimsumGS Σ).
   pose (F := (λ σ_t σ_s,
                ∀ n κs,
                ⌜σ_t ~{ m_trans m_t, κs, n }~>ₜ -⌝ -∗
